Fix stackWorld ordering bug

FunctionApp.v
@@ -2,21 +2,17 @@ Section process.
   Context {input : Type}.
   Context {world : Type}.
 
-  CoInductive process :=
-  | Step : (input -> (world -> world) * process) -> process.
-
   Definition action := world -> world.
-  Definition step := input -> action * process.
 
-  Definition runStep wp i :=
-    match wp with
-      | (w, Step pf) => let (a, p') := pf i in (a w, p')
-    end.
+  CoInductive process :=
+  | Step : (input -> action * process) -> process.
+
+  Definition step := input -> action * process.
 End process.
 
+Arguments action : clear implicits.
 Arguments process : clear implicits.
 Arguments step : clear implicits.
-Arguments action : clear implicits.
 
 
 Section stackProcess.
@@ -25,25 +21,27 @@ Section stackProcess.
   Context {input : Type}.
   Context {world : Type}.
 
-  Definition stackWorld := (list message * action world)%type.
+  Inductive stackWorld :=
+  | stackDone : stackWorld
+  | stackPush : message -> action stackWorld
+  | stackLift : action world -> action stackWorld.
+
   Definition stackInput := (message + input)%type.
   Definition stackProcess := process stackInput stackWorld.
   Definition stackStep := step stackInput stackWorld.
 
-  Definition stackPush (m : message) : action stackWorld :=
-    fun sw => let (ms, a) := sw in ((m :: ms)%list, a).
-  Definition stackLift (a : action world) : action stackWorld :=
-    fun sw => let (ms, a') := sw in (ms, fun w => a (a' w)).
-
   Definition stackTransition (m : stackInput) (pf : stackStep) :=
-    (fst (fst (pf m) (nil, @id world)), snd (pf m)).
+    (fst (pf m) stackDone, snd (pf m)).
 
-  Inductive emptiesStack : list message * stackProcess -> stackProcess -> Prop :=
-  | stackEmpty p : emptiesStack (nil, p) p
-  | popsStack (m : message) (ms : list message) (pf : stackStep) (p2 p3 : stackProcess) :
+  Inductive emptiesStack : stackWorld * stackProcess -> stackProcess -> Prop :=
+  | emptiesStackDone p : emptiesStack (stackDone, p) p
+  | emptiesStackPush m sw pf p2 p3 :
       emptiesStack (stackTransition (inl m) pf) p2 ->
-      emptiesStack (ms, p2) p3 ->
-      emptiesStack ((m :: ms)%list, Step pf) p3.
+      emptiesStack (sw, p2) p3 ->
+      emptiesStack (stackPush m sw, Step pf) p3
+  | emptiesStackLift a sw p p2 :
+      emptiesStack (sw, p) p2 ->
+      emptiesStack (stackLift a sw, p) p2.
 
   CoInductive emptiesStackForever : stackProcess -> Prop :=
   | emptiesStackStep pf p' :
@@ -52,21 +50,25 @@ Section stackProcess.
          emptiesStackForever (p' i)) ->
       emptiesStackForever (Step pf).
 
-  Inductive stepStackProcessTerminates : list message * stackProcess -> Prop :=
-  | stepStackProcessDone p : stepStackProcessTerminates (nil, p)
-  | stepStackProcessStep m ms pf p2 :
+  Inductive stepStackProcessTerminates : stackWorld * stackProcess -> Prop :=
+  | stepStackProcessDone p : stepStackProcessTerminates (stackDone, p)
+  | stepStackProcessPush m sw pf p2 :
       stepStackProcessTerminates (stackTransition (inl m) pf) ->
       emptiesStack (stackTransition (inl m) pf) p2 ->
-      stepStackProcessTerminates (ms, p2) ->
-      stepStackProcessTerminates ((m :: ms)%list, Step pf).
+      stepStackProcessTerminates (sw, p2) ->
+      stepStackProcessTerminates (stackPush m sw, Step pf)
+  | stepStackProcessLift a sw p p2 :
+      stepStackProcessTerminates (sw, p) ->
+      emptiesStack (sw, p) p2 ->
+      stepStackProcessTerminates (stackLift a sw, p).
 
-  Fixpoint mkStepStackProcessTerminates mp p' (e : emptiesStack mp p') : stepStackProcessTerminates mp.
-  destruct e; econstructor; eauto.
-  Defined.
+  Theorem mkStepStackProcessTerminates swp p' (e : emptiesStack swp p') : stepStackProcessTerminates swp.
+    induction e; econstructor; eauto.
+  Qed.
 
-  Fixpoint stepStackProcess mp (h : stepStackProcessTerminates mp) :
-    action world * sig (unique (emptiesStack mp)).
-  destruct mp as [[| m ms] p].
+  Fixpoint stepStackProcess swp (h : stepStackProcessTerminates swp) :
+    action world * sig (unique (emptiesStack swp)).
+  destruct swp as [[| m sw' | a sw'] p].
   {
     split.
     { exact (@id world). }
@@ -83,17 +85,17 @@ Section stackProcess.
   {
     destruct p as [pf].
     pose (sap1 := pf (inl m)).
-    pose (sw := fst sap1 (nil, @id world)).
-    assert (stepStackProcessTerminates (fst sw, snd sap1)) as e1 by (inversion h; assumption).
-    destruct (stepStackProcess (fst sw, snd sap1) e1) as [a2 [p2 [e2 u2]]].
-    assert (stepStackProcessTerminates (ms, p2)) as e3.
+    pose (sw := fst sap1 stackDone).
+    assert (stepStackProcessTerminates (sw, snd sap1)) as e1 by (inversion h; assumption).
+    destruct (stepStackProcess (sw, snd sap1) e1) as [a2 [p2 [e2 u2]]].
+    assert (stepStackProcessTerminates (sw', p2)) as e3.
     {
-      inversion h as [| ? ? ? p'].
+      inversion h as [| ? ? ? p' |].
       rewrite (u2 p'); assumption.
     }
-    destruct (stepStackProcess (ms, p2) e3) as [a3 [p3 [e4 u4]]].
+    destruct (stepStackProcess (sw', p2) e3) as [a3 [p3 [e4 u4]]].
     split.
-    { exact (fun w => a3 (a2 (snd sw w))). }
+    { exact (fun w => a3 (a2 w)). }
     {
       exists p3.
       split.
@@ -101,8 +103,25 @@ Section stackProcess.
       {
         intros p3' e5.
         apply u4.
-        inversion e5 as [| ? ? ? p'].
+        inversion e5 as [| ? ? ? p' |].
         rewrite (u2 p'); assumption.
+      }
+    }
+  }
+  {
+    assert (stepStackProcessTerminates (sw', p)) as e1 by (inversion h; assumption).
+    destruct (stepStackProcess (sw', p) e1) as [a2 [p2 [e2 u2]]].
+    split.
+    { exact (fun w => a2 (a w)). }
+    {
+      exists p2.
+      split.
+      { constructor. assumption. }
+      {
+        intros p2' h1.
+        apply u2.
+        inversion h1.
+        assumption.
       }
     }
   }
@@ -113,20 +132,20 @@ Section stackProcess.
   intro i.
   destruct p as [pf].
   pose (sap1 := pf (inr i)).
-  pose (sw := fst sap1 (nil, @id world)).
-  assert (stepStackProcessTerminates (fst sw, snd sap1)) as e1.
+  pose (sw := fst sap1 stackDone).
+  assert (stepStackProcessTerminates (sw, snd sap1)) as e1.
   {
     inversion h as [? ? h1].
     destruct (h1 i).
     eapply mkStepStackProcessTerminates.
     eassumption.
   }
-  destruct (stepStackProcess (fst sw, snd sap1) e1) as [a2 [p2 [e2 u2]]].
+  destruct (stepStackProcess (sw, snd sap1) e1) as [a2 [p2 [e2 u2]]].
   split.
-  { exact (fun w => a2 (snd sw w)). }
+  { exact a2. }
   {
     apply (runStackProcess p2).
-    inversion h as [? ? h1].
+    inversion h as [? p' h1].
     destruct (h1 i).
     rewrite (u2 (p' i)); assumption.
   }
